PossiblyInfiniteTrees/PossiblyInfiniteList/PossiblyInfiniteList.lean
@@ -1,4 +1,6 @@
-import PossiblyInfiniteTrees.PossiblyInfiniteList.InfiniteList
+module
+
+public import PossiblyInfiniteTrees.PossiblyInfiniteList.InfiniteList
 
 /-!
 # PossiblyInfiniteList
@@ -12,8 +14,12 @@ This file defines a `PossiblyInfiniteList` which is an `InfiniteList` over an `O
 The offered functions are very similar to the ones of `InfiniteList`.
 -/
 
+public section
+
 /-- An `InfiniteList` over `Option` has `no_holes` if an element being `none` implies its successors also being `none`. This is a property that we want for possibly infinite lists but we need to be able to express it on the underlying infinite list first. -/
-def InfiniteList.no_holes (l : InfiniteList (Option α)) : Prop := ∀ n : Nat, l.get n = none -> l.get n.succ = none
+@[expose]
+def InfiniteList.no_holes (l : InfiniteList (Option α)) : Prop :=
+  ∀ n : Nat, l.get n = none -> l.get n.succ = none
 
 /-- A `PossiblyInfiniteList` is an `InfiniteList` over `Option` that has `no_holes`. -/
 structure PossiblyInfiniteList (α : Type u) where
@@ -31,6 +37,7 @@ The essential functions on infinite lists, mainly get, drop, head, and tail.
 -/
 
 /-- Obtains the nth element from the list. -/
+@[expose]
 def get? (l : PossiblyInfiniteList α) (n : Nat) : Option α := l.infinite_list.get n
 
 /-- Obtain another possibly infinite list by dropping the first n elements from the current one. -/
@@ -39,6 +46,7 @@ def drop (l : PossiblyInfiniteList α) (n : Nat) : PossiblyInfiniteList α where
   no_holes := by intro n'; rw [InfiniteList.get_drop, InfiniteList.get_drop, Nat.add_succ]; exact l.no_holes (n + n')
 
 /-- Returns the first element. -/
+@[expose]
 def head (l : PossiblyInfiniteList α) : Option α := l.infinite_list.head
 
 /-- Drops the first element. -/
@@ -52,10 +60,9 @@ def cons (hd : α) (tl : PossiblyInfiniteList α) : PossiblyInfiniteList α wher
   no_holes := by
     intro n
     cases n with
-    | zero => intro contra; rw [← InfiniteList.head.eq_def, InfiniteList.head_cons] at contra; simp at contra
+    | zero => simp
     | succ n =>
-      rw [← InfiniteList.tail.eq_def, InfiniteList.tail_cons]
-      rw [← InfiniteList.tail.eq_def, InfiniteList.tail_cons]
+      simp only [InfiniteList.get_cons_succ]
       exact tl.no_holes n
 
 instance : Membership α (PossiblyInfiniteList α) where
@@ -65,18 +72,16 @@ instance : Membership α (PossiblyInfiniteList α) where
 theorem mem_iff {l : PossiblyInfiniteList α} : ∀ {e}, e ∈ l ↔ ∃ n, l.get? n = some e := by rfl
 
 /-- Two possibly infinite lists are the same of they are the same on all indices. -/
+@[ext, grind ext]
 theorem ext {l1 l2 : PossiblyInfiniteList α} : (∀ n, l1.get? n = l2.get? n) -> l1 = l2 := by
   intro h; rw [PossiblyInfiniteList.mk.injEq]; apply InfiniteList.ext; exact h
 
-theorem ext_iff {l1 l2 : PossiblyInfiniteList α} : l1 = l2 ↔ (∀ n, l1.get? n = l2.get? n) := by
-  constructor
-  . intro h _; rw [h]
-  . exact ext
-
 /-- `InfiniteList.no_holes` restated for the `PossiblyInfiniteList`. -/
+@[grind ->]
 theorem no_holes' {l : PossiblyInfiniteList α} : ∀ n, l.get? n = none -> l.get? n.succ = none := by exact l.no_holes
 
 /-- A closed version of the `no_holes` property. That is, if an element is none, then not only its immediate successor but all successors are none. -/
+@[grind ->]
 theorem get?_eq_none_of_le_of_eq_none {l : PossiblyInfiniteList α} {n : Nat} :
     l.get? n = none -> ∀ m, n ≤ m -> l.get? m = none := by
   intro h
@@ -91,42 +96,54 @@ theorem get?_eq_none_of_le_of_eq_none {l : PossiblyInfiniteList α} {n : Nat} :
   exact this k
 
 /-- Get after drop can be rewritten into get. -/
-theorem get?_drop {l : PossiblyInfiniteList α} {n i : Nat} : (l.drop n).get? i = l.get? (n + i) := by rfl
+@[simp, grind =]
+theorem get?_drop {l : PossiblyInfiniteList α} {n i : Nat} : (l.drop n).get? i = l.get? (n + i) := InfiniteList.get_drop
 
 /-- Dropping zero elements changes nothing. -/
+@[simp, grind =]
 theorem drop_zero {l : PossiblyInfiniteList α} : l.drop 0 = l := by
   rw [PossiblyInfiniteList.mk.injEq]; exact InfiniteList.drop_zero
 
 /-- The head is the same as getting the element at index zero. -/
-theorem head_eq {l : PossiblyInfiniteList α} : l.head = l.get? 0 := by rfl
+theorem head_eq {l : PossiblyInfiniteList α} : l.head = l.get? 0 := by unfold head; rw [InfiniteList.head_eq]; rfl
 
 /-- The `head` is in the list. -/
-theorem head_mem {l : PossiblyInfiniteList α} : ∀ h ∈ l.head, h ∈ l := by intro h h_mem; rw [Option.mem_def] at h_mem; simp only [Membership.mem, ← h_mem]; exact l.infinite_list.head_mem
+@[grind ->]
+theorem head_mem {l : PossiblyInfiniteList α} : ∀ h ∈ l.head, h ∈ l := by
+  intro h h_mem; rw [Option.mem_def] at h_mem; simp only [Membership.mem, ← h_mem]; exact l.infinite_list.head_mem
 
 /-- Getting the head after dropping n equals getting n. -/
-theorem head_drop {l : PossiblyInfiniteList α} : ∀ {n}, (l.drop n).head = l.get? n := by intros; rfl
+@[simp, grind =]
+theorem head_drop {l : PossiblyInfiniteList α} : ∀ {n}, (l.drop n).head = l.get? n := InfiniteList.head_drop
 
 /-- Getting the nth element from the tail equals getting the successor of n from the original list. -/
-theorem get?_tail {l : PossiblyInfiniteList α} : ∀ n, l.tail.get? n = l.get? n.succ := by intros; rfl
+@[simp, grind =]
+theorem get?_tail {l : PossiblyInfiniteList α} : ∀ n, l.tail.get? n = l.get? n.succ := InfiniteList.get_tail
 
 /-- Getting the tail after dropping n is the same as dropping n.succ. -/
+@[simp, grind =]
 theorem tail_drop {l : PossiblyInfiniteList α} : ∀ {n}, (l.drop n).tail = l.drop n.succ := by
-  intros; unfold tail drop; apply ext; intro n; simp only [get?, InfiniteList.tail_drop]
+  intros; unfold tail drop; ext; simp
 
 /-- Getting the first element on cons is the new head. -/
-theorem get?_cons_zero {hd : α} {tl : PossiblyInfiniteList α} : (cons hd tl).get? 0 = .some hd := by unfold get?; unfold cons; rw [InfiniteList.get_cons_zero]
+@[simp, grind =]
+theorem get?_cons_zero {hd : α} {tl : PossiblyInfiniteList α} : (cons hd tl).get? 0 = .some hd := by simp [get?, cons]
 
 /-- Getting any index > 0 on cons yields the respective element from the previous possibly infinite list. -/
-theorem get?_cons_succ {hd : α} {tl : PossiblyInfiniteList α} : ∀ n, (cons hd tl).get? n.succ = tl.get? n := by intro n; unfold get?; unfold cons; rw [InfiniteList.get_cons_succ]
+@[simp, grind =]
+theorem get?_cons_succ {hd : α} {tl : PossiblyInfiniteList α} : ∀ n, (cons hd tl).get? n.succ = tl.get? n := by simp [get?, cons]
 
 /-- The `head` of `cons` is the head used in the construction. -/
+@[simp, grind =]
 theorem head_cons (hd : α) (tl : PossiblyInfiniteList α) : (cons hd tl).head = hd := InfiniteList.head_cons
 
 /-- The `tail` of `cons` is the list used in the construction. -/
-theorem tail_cons (hd : α) (tl : PossiblyInfiniteList α) : (cons hd tl).tail = tl := by simp [cons, tail, InfiniteList.tail_cons]
+@[simp, grind =]
+theorem tail_cons (hd : α) (tl : PossiblyInfiniteList α) : (cons hd tl).tail = tl := by simp [cons, tail]
 
 /-- Any `PossiblyInfiniteList` can be written using the `cons` constructor. -/
-theorem cons_head_tail (l : PossiblyInfiniteList α) (hd : α) (h : l.head = .some hd) : l = cons hd l.tail := by rw [PossiblyInfiniteList.mk.injEq]; simp only [cons]; rw [← h]; apply InfiniteList.cons_head_tail
+theorem cons_head_tail (l : PossiblyInfiniteList α) (hd : α) (h : l.head = .some hd) : l = cons hd l.tail := by
+  rw [PossiblyInfiniteList.mk.injEq]; simp only [cons]; rw [← h]; apply InfiniteList.cons_head_tail
 
 end Basic
 
@@ -147,27 +164,33 @@ infixl:50 " <:+ " => IsSuffix
 
 /-- l1 is a suffix of l2 if l1 can be obtained from l2 by dropping some elements. -/
 theorem IsSuffix_iff {l1 l2 : PossiblyInfiniteList α} : l1 <:+ l2 ↔ ∃ n, l2.drop n = l1 := by
+  unfold IsSuffix; rw [InfiniteList.IsSuffix_iff]
   constructor
   . rintro ⟨n, h⟩; exists n; simp [drop, h]
-  . rintro ⟨n, h⟩; exists n; simp only [drop] at h; rw [← h]
+  . rintro ⟨n, h⟩; exists n; rw [← h]; simp [drop]
 
 /-- The suffix relation is reflexive. -/
+@[grind <-]
 theorem IsSuffix_refl {l : PossiblyInfiniteList α} : l <:+ l := l.infinite_list.IsSuffix_refl
 
 /-- The suffix relation is transitive. -/
+@[grind ->]
 theorem IsSuffix_trans {l1 l2 l3 : PossiblyInfiniteList α} : l1 <:+ l2 -> l2 <:+ l3 -> l1 <:+ l3 := InfiniteList.IsSuffix_trans
 
 /-- Two suffixes of the same list must be suffixes of each other in some way. This is similar to List.suffix_or_suffix_of_suffix. -/
 theorem suffix_or_suffix_of_suffix {l1 l2 l3 : PossiblyInfiniteList α} : l1 <:+ l3 -> l2 <:+ l3 -> (l1 <:+ l2) ∨ (l2 <:+ l1) := InfiniteList.suffix_or_suffix_of_suffix
 
 /-- A member of a suffix is also a member of the current list. -/
+@[grind ->]
 theorem mem_of_mem_suffix {l1 l2 : PossiblyInfiniteList α} (suffix : l1 <:+ l2) : ∀ e ∈ l1, e ∈ l2 := by
   intro e mem; apply InfiniteList.mem_of_mem_suffix suffix; exact mem
 
 /-- Dropping elements yields a suffix. -/
+@[grind <-]
 theorem IsSuffix_drop {l : PossiblyInfiniteList α} : ∀ n, l.drop n <:+ l := l.infinite_list.IsSuffix_drop
 
 /-- The `tail` is a suffix. -/
+@[grind <-]
 theorem IsSuffix_tail {l : PossiblyInfiniteList α} : l.tail <:+ l := l.infinite_list.IsSuffix_tail
 
 end Suffixes
@@ -183,6 +206,7 @@ Note that for using this coveniently, the goal needs to expressed (rewritten) us
 -/
 
 /-- A list `Element` is a Subtype featuring a proof of being a list member. -/
+@[expose]
 def Element (l : PossiblyInfiniteList α) := { e : α // e ∈ l }
 
 /-- A recursor for proving properties about list members via induction. -/
@@ -199,15 +223,15 @@ theorem mem_rec
     induction a' using InfiniteList.mem_rec with
     | head => exact head
     | step l2 suffix ih =>
+      rw [InfiniteList.IsSuffix_iff] at suffix
       rcases suffix with ⟨n, suffix⟩
       simp only [← suffix]
       cases eq : (l.infinite_list.drop n).head with
-      | none => simp only [InfiniteList.head_drop, InfiniteList.tail_drop, motive']; intro _ mem; rw [Option.mem_def, l.no_holes] at mem; simp at mem; exact eq
+      | none => simp only [InfiniteList.head_drop, InfiniteList.tail_drop, motive']; intro _ mem; rw [Option.mem_def, l.no_holes] at mem; simp at mem; grind
       | some b =>
         specialize step (l.drop n) (l.IsSuffix_drop n)
         apply step
         exists b, eq
-        unfold motive' at ih
         apply ih
         simp only [← suffix]
         exact eq
@@ -230,19 +254,47 @@ def map (l : PossiblyInfiniteList α) (f : α -> β) : PossiblyInfiniteList β w
   no_holes := by intro n; simp only [InfiniteList.get_map, Option.map_eq_none_iff]; apply l.no_holes
 
 /-- When getting after map, we can instead get and then apply the mapping function. -/
-theorem get?_map {l : PossiblyInfiniteList α} {f : α -> β} {n : Nat} : (l.map f).get? n = (l.get? n).map f := by rfl
+@[simp, grind =]
+theorem get?_map {l : PossiblyInfiniteList α} {f : α -> β} {n : Nat} : (l.map f).get? n = (l.get? n).map f := InfiniteList.get_map
 
 /-- An element `e` is in the mapped list if there was an element that maps to `e`. -/
+@[simp]
 theorem mem_map {l : PossiblyInfiniteList α} {f : α -> β} : ∀ e, e ∈ (l.map f) ↔ ∃ e' ∈ l, f e' = e := by
   intro e
+  rw [mem_iff]
   constructor
-  . rintro ⟨i, e_mem⟩; rw [← PossiblyInfiniteList.get?.eq_def, get?_map, Option.map_eq_some_iff] at e_mem; rcases e_mem with ⟨e', e'_mem, e_eq⟩; exists e'; constructor; exists i; exact e_eq
-  . rintro ⟨e', ⟨i, e'_mem⟩, e_eq⟩; rw [← e_eq]; exists i; rw [← PossiblyInfiniteList.get?.eq_def, get?_map, Option.map_eq_some_iff]; exists e'
+  . rintro ⟨i, e_mem⟩; rw [get?_map, Option.map_eq_some_iff] at e_mem; rcases e_mem with ⟨e', e'_mem, e_eq⟩; exists e'; constructor; exists i; exact e_eq
+  . rintro ⟨e', ⟨i, e'_mem⟩, e_eq⟩; rw [← e_eq]; exists i; rw [get?_map, Option.map_eq_some_iff]; exists e'
+
+/-- The head of a mapped list is the same as applying the function to the head. -/
+@[simp, grind =]
+theorem head_map {l : PossiblyInfiniteList α} {f : α -> β} : (l.map f).head = l.head.map f := InfiniteList.head_map
 
 /-- The tail of a mapped list is the same as applyign map to the tail. -/
-theorem tail_map {l : PossiblyInfiniteList α} {f : α -> β} : (l.map f).tail = l.tail.map f := by rfl
+@[simp, grind =]
+theorem tail_map {l : PossiblyInfiniteList α} {f : α -> β} : (l.map f).tail = l.tail.map f := by ext; simp
 
 end Map
+
+
+section Attach
+
+/-!
+## Attach
+
+We allow to `attach` membership proofs to list elements just like `List.attach`.
+-/
+
+/-- Attaches a membership proof to each list element. -/
+def attach (l : PossiblyInfiniteList α) : PossiblyInfiniteList l.Element where
+  infinite_list := l.infinite_list.attach.map (fun e => e.val.attach.map (fun v => ⟨v.val, by rw [mem_iff]; rcases e.property with ⟨n, eq⟩; exists n; simp only [get?]; rw [eq]; exact v.property⟩))
+  no_holes := by intro n; simpa using l.no_holes n
+
+/-- Calling `get` after `attach` returns the correct element with its membership proof. -/
+theorem val_get_attach {l : PossiblyInfiniteList α} :
+  ∀ {n}, (l.attach.get? n).map (fun e => e.val) = l.get? n := by intros; simp [get?, attach]
+
+end Attach
 
 section Generate
 
@@ -263,20 +315,24 @@ def generate (start : Option α) (generator : α -> Option α) (mapper : α -> �
 }
 
 /-- The head of a generated list is the mapped version of the starting value. -/
-theorem head_generate {start : Option α} {generator : α -> Option α} {mapper : α -> β} : (generate start generator mapper).head = start.map mapper := rfl
+@[simp, grind =]
+theorem head_generate {start : Option α} {generator : α -> Option α} {mapper : α -> β} :
+  (generate start generator mapper).head = start.map mapper := InfiniteList.head_generate
 
 /-- The nth element of a generated list is the mapped version of the nth element of the iterated "carrier" list. -/
 theorem get?_generate {start : Option α} {generator : α -> Option α} {mapper : α -> β} :
-  ∀ n, (generate start generator mapper).get? n = ((InfiniteList.iterate start (·.bind generator)).get n).map mapper := by intros; rfl
+  ∀ n, (generate start generator mapper).get? n = ((InfiniteList.iterate start (·.bind generator)).get n).map mapper := InfiniteList.get_generate
 
 /-- The successor of the nth element of a generated list can be seen as applying the mapper function after the generator function after taking the nth element from the iterated "carrier" list. -/
 theorem get?_succ_generate {start : Option α} {generator : α -> Option α} {mapper : α -> β} :
-  ∀ n, (generate start generator mapper).get? n.succ = (((InfiniteList.iterate start (·.bind generator)).get n).bind generator).map mapper := by intros; rfl
+    ∀ n, (generate start generator mapper).get? n.succ = (((InfiniteList.iterate start (·.bind generator)).get n).bind generator).map mapper :=
+  InfiniteList.get_succ_generate
 
 /-- The tail of a generated list is the list generated when applying the generator function once on the starting element before the actual generation. -/
-theorem tail_generate {start : Option α} {generator : α -> Option α} {mapper : α -> β} : (generate start generator mapper).tail = generate (start.bind generator) generator mapper := by
+theorem tail_generate {start : Option α} {generator : α -> Option α} {mapper : α -> β} :
+    (generate start generator mapper).tail = generate (start.bind generator) generator mapper := by
   simp only [generate, tail, mk.injEq]
-  rw [InfiniteList.tail_generate]
+  exact InfiniteList.tail_generate
 
 end Generate
 
@@ -291,20 +347,30 @@ The `empty` `PossiblyInfiniteList` is simply the `PossiblyInfiniteList` that is 
 /-- The empty `PossiblyInfiniteList` is none everywhere. -/
 def empty : PossiblyInfiniteList α where
   infinite_list := fun _ => none
-  no_holes := by intro _ _; rfl
+  no_holes := by intro _ _; rw [InfiniteList.compute_get]
 
 /-- Getting from the empty list always returns none. -/
-theorem get?_empty {α} : ∀ {n}, (@PossiblyInfiniteList.empty α).get? n = none := by intro _; rfl
+@[simp, grind =]
+theorem get?_empty {α} : ∀ {n}, (@PossiblyInfiniteList.empty α).get? n = none := by
+  intro _; unfold get?; rw [InfiniteList.compute_get]; rfl
+
+/-- The head of the empty list is none. -/
+@[simp, grind =]
+theorem head_empty {α} : (@PossiblyInfiniteList.empty α).head = none := by simp [head_eq]
+
+/-- The empty list stays empty when mapped. -/
+@[simp, grind =]
+theorem map_empty {α} {f : α -> β} : (@PossiblyInfiniteList.empty α).map f = empty := by ext; simp
 
 /-- A `PossiblyInfiniteList` is empty if and only if its head is none. -/
 theorem empty_iff_head_none {l : PossiblyInfiniteList α} : l = PossiblyInfiniteList.empty ↔ l.head = none := by
   constructor
-  . intro h; rw [h]; simp [head, empty, InfiniteList.head, InfiniteList.get]
+  . intro h; simp [h]
   intro h
   apply ext
   intro n
   induction n with
-  | zero => rw [get?_empty]; exact h
+  | zero => rw [get?_empty, ← head_eq]; exact h
   | succ n ih =>
     rw [get?_empty] at ih
     rw [get?_empty]
@@ -323,6 +389,7 @@ We also define a function converting a `finite` `PossiblyInfiniteList` into a pl
 -/
 
 /-- The `PossiblyInfiniteList` is finite if some element is none. -/
+@[expose]
 def finite (l : PossiblyInfiniteList α) : Prop := ∃ k, l.get? k = none
 
 /-- Transforms a finite list into an inductive `List`. -/
@@ -333,39 +400,33 @@ def toList_of_finite (l : PossiblyInfiniteList α) (fin : l.finite) : List α :=
     | .some a =>
       have termination_hint : Classical.choose fin - (n + 1) < Classical.choose fin - n := by
         apply Nat.sub_add_lt_sub _ (by simp)
-        have spec := Classical.choose_spec fin
-        apply Classical.byContradiction
-        intro contra
-        simp only [Nat.not_le] at contra
-        have contra := Nat.le_of_lt_succ contra
-        have := l.get?_eq_none_of_le_of_eq_none spec _ contra
-        rw [eq] at this
-        simp at this
+        grind
       a :: loop (n+1)
   termination_by (Classical.choose fin) - n
   loop 0
 
 /-- A mapped list is finite if the original list is finite. -/
+@[grind <-]
 theorem map_finite_of_finite {l : PossiblyInfiniteList α} {f : α -> β} : l.finite -> (l.map f).finite := by
-  rintro ⟨i, h⟩; exists i; rw [get?_map, Option.map_eq_none_iff]; exact h
+  rintro ⟨i, _⟩; exists i; grind
 
 /-- The empty list is finite. -/
-theorem finite_empty {α} : (@PossiblyInfiniteList.empty α).finite := by exists 0
+@[grind <-]
+theorem finite_empty {α} : (@PossiblyInfiniteList.empty α).finite := by exists 0; simp
 
 /-- The nth element in the transformed list is the nth element from the original list. -/
+@[simp, grind =]
 theorem getElem?_toList_of_finite {l : PossiblyInfiniteList α} {fin : l.finite} : ∀ {n}, (l.toList_of_finite fin)[n]? = l.get? n := by
   have : ∀ n m, (toList_of_finite.loop l fin m)[n]? = l.get? (m + n) := by
     intro n
     induction n with
     | zero =>
-      intro m; unfold toList_of_finite.loop
-      split
-      case h_1 eq => simp [eq]
-      case h_2 eq => simp [eq]
+      unfold toList_of_finite.loop
+      grind
     | succ n ih =>
       intro m; unfold toList_of_finite.loop; specialize ih (m+1); rw [Nat.add_comm n 1, ← Nat.add_assoc, ← ih]
       split
-      case h_2 eq => rw [Nat.add_comm 1 n, List.getElem?_cons_succ]
+      case h_2 eq => grind
       case h_1 eq =>
         unfold toList_of_finite.loop
         split
@@ -380,37 +441,29 @@ theorem getElem?_toList_of_finite {l : PossiblyInfiniteList α} {fin : l.finite}
   rw [this n 0, Nat.zero_add]
 
 /-- An element is in the transformed finite list if and only if it is in the original list. -/
+@[simp, grind =]
 theorem mem_toList_of_finite {l : PossiblyInfiniteList α} {fin : l.finite} : ∀ {e}, e ∈ l.toList_of_finite fin ↔ e ∈ l := by
   intro e
-  rw [List.mem_iff_getElem?]
-  constructor
-  . intro h; rcases h with ⟨i, h⟩; exists i; rw [getElem?_toList_of_finite] at h; exact h
-  . intro h; rcases h with ⟨i, h⟩; exists i; rw [getElem?_toList_of_finite]; exact h
+  rw [List.mem_iff_getElem?, mem_iff]
+  constructor <;> (intro h; rcases h with ⟨i, h⟩; exists i; grind)
 
 /-- Mapping over the transformed finite list is the same as mapping first and then transforming. -/
-theorem map_toList_of_finite {l : PossiblyInfiniteList α} {fin : l.finite} {f : α -> β} : (l.toList_of_finite fin).map f = (l.map f).toList_of_finite (map_finite_of_finite fin) := by
-  apply List.ext_getElem?
-  intro i
-  rw [List.getElem?_map, getElem?_toList_of_finite, getElem?_toList_of_finite]
-  rfl
+@[simp, grind =]
+theorem map_toList_of_finite {l : PossiblyInfiniteList α} {fin : l.finite} {f : α -> β} :
+  (l.toList_of_finite fin).map f = (l.map f).toList_of_finite (map_finite_of_finite fin) := by apply List.ext_getElem?; simp
 
 /-- The transformed list is empty if and only if the original list is empty. -/
 theorem toList_of_finite_empty_iff {l : PossiblyInfiniteList α} {fin : l.finite} : l.toList_of_finite fin = [] ↔ l = PossiblyInfiniteList.empty := by
   constructor
   . intro eq
-    apply PossiblyInfiniteList.ext
     rw [List.ext_getElem?_iff] at eq
+    apply PossiblyInfiniteList.ext
     intro n
     specialize eq n
-    rw [getElem?_toList_of_finite] at eq
-    rw [eq]
-    rfl
+    grind
   . intro eq
     apply List.ext_getElem?
-    intro n
-    rw [getElem?_toList_of_finite]
-    rw [eq]
-    rw [get?_empty, List.getElem?_nil]
+    simp [eq]
 
 end Finite
 
@@ -425,17 +478,19 @@ We can always convert a plain `List` into a `PossiblyInfiniteList` by setting al
 /-- Builds a PossiblyInfiniteList from an inductive `List`. -/
 def from_list (l : List α) : PossiblyInfiniteList α where
   infinite_list := fun n => l[n]?
-  no_holes := by intro n; simp only [InfiniteList.get]; simp only [List.getElem?_eq_none_iff]; exact Nat.le_succ_of_le
+  no_holes := by intro n; simp only [InfiniteList.compute_get]; simp only [List.getElem?_eq_none_iff]; exact Nat.le_succ_of_le
 
 /-- After building from a `List`, the nth elements are the same. -/
-theorem get?_from_list {l : List α} : ∀ {n}, (from_list l).get? n = l[n]? := by intros; rfl
+@[simp, grind =]
+theorem get?_from_list {l : List α} : ∀ {n}, (from_list l).get? n = l[n]? := by intros; unfold from_list get?; rw [InfiniteList.compute_get]
 
 /-- When building from a `List`, the `PossiblyInfiniteList` is `finite`. -/
-theorem finite_from_list {l : List α} : (from_list l).finite := by exists l.length; rw [get?_from_list]; apply List.getElem?_eq_none; simp
+@[grind <-]
+theorem finite_from_list {l : List α} : (from_list l).finite := by exists l.length; simp
 
 /-- Transforming a `List` to a `PossiblyInfiniteList` and back, gives the original list. -/
-theorem toList_of_finite_after_from_list {l : List α} : (from_list l).toList_of_finite finite_from_list = l := by
-  apply List.ext_getElem?; intro i; rw [getElem?_toList_of_finite, get?_from_list]
+@[simp, grind =]
+theorem toList_of_finite_after_from_list {l : List α} : (from_list l).toList_of_finite finite_from_list = l := by ext; simp
 
 end FromList
 
